----------------------------------------------------------------------
Committing in a revised version of the quotients package, where now
erroneous input theorems are usually detected early, and the erroneous
theorem listed in an error message.  This should greatly improve the
usability of the package, especially for new users.  Thanks to Michael
Norrish for prodding me on this one.

Also added a new version of finite sets from lists, due to Michael Norrish.

Also moved the "obj" directory to now be called "sigma"; this contains
the sigma calculus example from Abadi and Cardelli, as described in the
longer 45-page paper.

Modified Files:
	hol98/src/quotient/examples/finite_setScript.sml
	hol98/src/quotient/src/quotient.sml
	hol98/src/quotient/src/quotientScript.sml
Added Files:
	hol98/src/quotient/examples/ext_finite_setScript.sml
	hol98/src/quotient/examples/sigma/MutualIndThen.sig
	hol98/src/quotient/examples/sigma/MutualIndThen.sml
	hol98/src/quotient/examples/sigma/alphaScript.sml
	hol98/src/quotient/examples/sigma/barendregt.sig
	hol98/src/quotient/examples/sigma/barendregt.sml
	hol98/src/quotient/examples/sigma/ind_rel.sig
	hol98/src/quotient/examples/sigma/ind_rel.sml
	hol98/src/quotient/examples/sigma/liftScript.sml
	hol98/src/quotient/examples/sigma/more_listScript.sml
	hol98/src/quotient/examples/sigma/more_setScript.sml
	hol98/src/quotient/examples/sigma/objectScript.sml
	hol98/src/quotient/examples/sigma/reductionScript.sml
	hol98/src/quotient/examples/sigma/semanticsScript.sml
	hol98/src/quotient/examples/sigma/tactics.sig
	hol98/src/quotient/examples/sigma/tactics.sml
	hol98/src/quotient/examples/sigma/variableScript.sml
Removed Files:
	hol98/src/quotient/examples/obj/MutualIndThen.sig
	hol98/src/quotient/examples/obj/MutualIndThen.sml
	hol98/src/quotient/examples/obj/alphaScript.sml
	hol98/src/quotient/examples/obj/barendregt.sig
	hol98/src/quotient/examples/obj/barendregt.sml
	hol98/src/quotient/examples/obj/ind_rel.sig
	hol98/src/quotient/examples/obj/ind_rel.sml
	hol98/src/quotient/examples/obj/liftScript.sml
	hol98/src/quotient/examples/obj/more_listScript.sml
	hol98/src/quotient/examples/obj/more_setScript.sml
	hol98/src/quotient/examples/obj/objectScript.sml
	hol98/src/quotient/examples/obj/reductionScript.sml
	hol98/src/quotient/examples/obj/semanticsScript.sml
	hol98/src/quotient/examples/obj/tactics.sig
	hol98/src/quotient/examples/obj/tactics.sml
	hol98/src/quotient/examples/obj/variableScript.sml
----------------------------------------------------------------------

src/quotient/src/quotientScript.sml
@@ -54,6 +54,21 @@ val EQUIV_def =
     Define
       `EQUIV E = !x y:'a. E x y = (E x = E y)`;
 
+(* Partial Equivalence relations: *)
+
+val PARTIAL_EQUIV_def =
+    Define
+      `PARTIAL_EQUIV R = (?x:'a. R x x) /\
+                         (!x y.  R x y = R x x /\ R y y /\ (R x = R y))`;
+
+val EQUIV_IMP_PARTIAL_EQUIV = store_thm
+  ("EQUIV_IMP_PARTIAL_EQUIV",
+    (--`!R :'a -> 'a -> bool. EQUIV R ==> PARTIAL_EQUIV R`--),
+    REWRITE_TAC[EQUIV_def,PARTIAL_EQUIV_def]
+    THEN REPEAT STRIP_TAC
+    THEN PROVE_TAC[]
+   );
+
 (* Quotients, with partial equivalence relation, abstraction function, and
    representation function: *)
 
