src/quotient/examples/ext_finite_setScript.sml
@@ -1,0 +1,394 @@
+(* An alternative approach to creating finite sets as a quotient of lists.  *)
+(* This takes the extensionality principle as the definition of equivalence.*)
+(* Composed and contributed by Dr. Michael Norrish.                         *)
+(* June 24, 2005.                                                           *)
+
+open HolKernel Parse boolLib bossLib BasicProvers listTheory quotientLib
+
+val _ = new_theory "ext_finite_set";
+
+fun Store_Thm(n,t,tac) = store_thm(n,t,tac) before
+                         BasicProvers.export_rewrites [n]
+
+val leq_def = Define`leq x y = !e:'a. MEM e x = MEM e y`
+
+val leq_refl = Store_Thm(
+  "leq_refl",
+  ``!x :'a list. leq x x``,
+  SRW_TAC [] [leq_def]);
+
+val leq_sym = Store_Thm(
+  "leq_sym",
+  ``!x y :'a list. leq x y ==> leq y x``,
+  SRW_TAC [] [leq_def]);
+
+val leq_trans = Store_Thm(
+  "leq_trans",
+  ``!x y z :'a list. leq x y /\ leq y z ==> leq x z``,
+  SRW_TAC [] [leq_def]);
+
+(* functions on representatives *)
+
+(* insertion is represented by :: *)
+val NOT_NIL_EQUIV_CONS = store_thm(
+  "NOT_NIL_EQUIV_CONS",
+  ``~(leq [] ((a:'a)::A))``,
+  SRW_TAC [boolSimps.DNF_ss] [leq_def]);
+
+val NIL_RSP = store_thm(
+  "NIL_RSP",
+  ``leq ([]:'a list) []``,
+  SRW_TAC [] [leq_def]);
+
+val CONS_RSP = store_thm(
+  "CONS_RSP",
+  ``!x:'a A B. leq A B ==> leq (x::A) (x::B)``,
+  SRW_TAC [] [leq_def]);
+
+(* membership is represented by MEM *)
+val MEM_RSP = store_thm(
+  "MEM_RSP",
+  ``!X Y x:'a. leq X Y ==> (MEM x X = MEM x Y)``,
+  SRW_TAC [] [leq_def]);
+
+val NO_MEM_NIL = Store_Thm(
+  "NO_MEM_NIL",
+  ``!A. (!a:'a. ~(MEM a A)) = (A = [])``,
+  Induct_on `A` THEN SRW_TAC [] [] THEN PROVE_TAC []);
+
+val NONE_MEM_NIL = store_thm(
+  "NONE_MEM_NIL",
+  ``!A. (!a:'a. ~(MEM a A)) = (leq A [])``,
+  SRW_TAC [] [leq_def]);
+
+val MEM_CONS = store_thm(
+  "MEM_CONS",
+  ``!A (a:'a). MEM a A ==> leq (a :: A) A``,
+  SRW_TAC [] [leq_def] THEN PROVE_TAC []);
+
+val CONS_LEFT_COMM = prove(
+  ``!A x y:'a. leq (x::y::A) (y::x::A)``,
+  SRW_TAC [] [leq_def] THEN PROVE_TAC []);
+
+val CONS_LEFT_IDEM = prove(
+  ``!A x:'a. leq (x::x::A) (x::A)``,
+  SRW_TAC [] [leq_def] THEN PROVE_TAC []);
+
+val finite_set1_strong_cases = store_thm(
+  "finite_set1_strong_cases",
+  ``!X. (X = []) \/ ?(a:'a) Y. ~MEM a Y /\ leq X (a::Y)``,
+  Induct THEN FULL_SIMP_TAC (srw_ss()) [leq_def] THEN
+  METIS_TAC [MEM]);
+
+(* Delete1 *)
+val Delete1_def = Define
+   `($Delete1 [] x = [])  /\
+    ($Delete1 ((a:'a) :: A) x = if a = x then $Delete1 A x
+                                     else a :: ($Delete1 A x))`;
+val _ = export_rewrites ["Delete1_def"]
+
+val _ = add_infix ("Delete1", 500, HOLgrammars.LEFT);
+
+val MEM_Delete1 = store_thm (
+  "MEM_Delete1",
+  ``!A (a:'a) x. MEM x (A Delete1 a) = MEM x A /\ ~(x = a)``,
+  Induct THEN SRW_TAC[][] THEN PROVE_TAC []);
+
+val MEM_Delete1_IDENT = Store_Thm(
+  "MEM_Delete1_IDENT",
+  ``!A (a:'a). ~(MEM a (A Delete1 a))``,
+  Induct_on `A` THEN SRW_TAC [][]);
+
+val NOT_MEM_Delete1_IDENT = store_thm(
+  "NOT_MEM_Delete1_IDENT",
+  ``!A (b:'a). ~MEM b A ==> (A Delete1 b = A)``,
+  Induct_on `A` THEN SRW_TAC [][]);
+
+val Delete1_RSP = store_thm(
+  "Delete1_RSP",
+  ``!A B (a:'a). leq A B ==> (leq (A Delete1 a) (B Delete1 a))``,
+  SRW_TAC [] [leq_def,MEM_Delete1]);
+
+val CONS_Delete1 = store_thm(
+  "CONS_Delete1",
+  ``!A (a:'a). leq (a :: (A Delete1 a)) (if MEM a A then A else a::A)``,
+  SRW_TAC [] [leq_def, MEM_Delete1] THEN PROVE_TAC []);
+
+val MEM_CONS_Delete1 = store_thm
+   ("MEM_CONS_Delete1",
+    ``!A (a:'a). MEM a A ==> leq (a :: (A Delete1 a)) A``,
+    PROVE_TAC [CONS_Delete1]
+   );
+
+val finite_set1_Delete1_cases1 = store_thm
+   ("finite_set1_Delete1_cases1",
+    ``!X. (X = []) \/ ?a:'a. leq X (a :: (X Delete1 a))``,
+    Cases THEN SRW_TAC [][leq_def, MEM_Delete1] THEN METIS_TAC []);
+
+val finite_set1_Delete1_cases = store_thm
+   ("finite_set1_Delete1_cases",
+    ``!X. (X = []) \/
+            ?a:'a. MEM a X /\ leq X (a :: (X Delete1 a))``,
+    PROVE_TAC[finite_set1_Delete1_cases1,MEM,MEM_RSP]
+   );
+
+(* Card1 *)
+
+val Card1_def = Define
+   `(Card1 ([]) = 0)  /\
+    (Card1 ((a:'a) :: A) = if MEM a A then Card1 A else SUC (Card1 A))`;
+val _ = export_rewrites ["Card1_def"]
+
+val NOT_MEM_Card1 = store_thm
+   ("NOT_MEM_Card1",
+    ``!A:'a list a. ~(MEM a A) ==>
+             (Card1 (a :: A) = SUC (Card1 A))``,
+    RW_TAC std_ss [Card1_def]
+   );
+
+val Card1_SUC = store_thm (
+  "Card1_SUC",
+  ``!A n. (Card1 A = SUC n) ==>
+          ?(a:'a) B. ~(MEM a B) /\ leq A (a :: B)``,
+  Induct THEN SRW_TAC [][] THENL [
+    PROVE_TAC [MEM_CONS, leq_trans, leq_sym],
+    PROVE_TAC [leq_refl]
+  ]);
+
+val MEM_Card1_NOT_0 = store_thm(
+  "MEM_Card1_NOT_0",
+  ``!A a. MEM (a:'a) A ==> ~(Card1 A = 0)``,
+  Induct_on `A` THEN SRW_TAC [][] THEN PROVE_TAC []);
+
+val Card1_CONS_GT_0 = store_thm (
+  "Card1_CONS_GT_0",
+  ``!A (a:'a). 0 < Card1 (a :: A)``,
+  METIS_TAC [MEM, arithmeticTheory.NOT_ZERO_LT_ZERO,
+             MEM_Card1_NOT_0]);
+
+val Card1_Delete1 = store_thm(
+  "Card1_Delete1",
+  ``!A (a:'a).
+      Card1 (A Delete1 a) = if MEM a A then Card1 A - 1 else Card1 A``,
+  Induct_on `A` THEN SRW_TAC [][MEM_Delete1] THEN SRW_TAC [][] THEN
+  PROVE_TAC [MEM_Card1_NOT_0, DECIDE ``~(x = 0) ==> (SUC (x - 1) = x)``]);
+
+val Card1_RSP = store_thm (
+  "Card1_RSP",
+  ``!A B:'a list. leq A B ==> (Card1 A = Card1 B)``,
+  SIMP_TAC (srw_ss()) [leq_def] THEN Induct THEN SRW_TAC [][] THENL [
+    PROVE_TAC [],
+    `MEM h B /\ ~(Card1 B = 0)` by PROVE_TAC [MEM_Card1_NOT_0] THEN
+    Q_TAC SUFF_TAC `Card1 A = Card1 (B Delete1 h)`
+          THEN1 SRW_TAC [numSimps.ARITH_ss][Card1_Delete1] THEN
+    FIRST_X_ASSUM MATCH_MP_TAC THEN SRW_TAC [][MEM_Delete1] THEN
+    PROVE_TAC []
+  ]);
+
+val Card1_0 = store_thm(
+  "Card1_0",
+  ``!A:'a list. (Card1 A = 0) = (A = [])``,
+  Induct_on `A` THEN SRW_TAC [][] THEN PROVE_TAC [NO_MEM_NIL]);
+
+(* list2set *)
+val list2set_thm = prove(
+  ``(LIST_TO_SET ([]:'a list) = {}) /\
+    (!h:'a t. LIST_TO_SET (h::t) = h INSERT LIST_TO_SET t)``,
+  SRW_TAC [][pred_setTheory.EXTENSION]);
+
+val list2set_RSP = store_thm(
+  "list2set_RSP",
+  ``!A B:'a list. leq A B ==> (LIST_TO_SET A = LIST_TO_SET B)``,
+  SRW_TAC [][leq_def, pred_setTheory.EXTENSION]);
+
+(* fold *)
+
+val Fold1_def = Define`
+  (Fold1 f (z:'b) [] = z) /\
+  (Fold1 f z ((a:'a)::A) =
+     if (!u v w. f u (f v w) = f v (f u w)) then
+       if MEM a A then Fold1 f z A
+       else f a (Fold1 f z A)
+     else z)
+` ;
+
+val MEM_lcommuting_Fold1 = store_thm(
+  "MEM_lcommuting_Fold1",
+  ``!B f (z:'b) (h:'a).
+     (!u v w. f u (f v w) = f v (f u w)) /\ MEM h B ==>
+     (Fold1 f z B = f h (Fold1 f z (B Delete1 h)))``,
+  Induct_on `B` THEN SRW_TAC [][Fold1_def, MEM_Delete1] THENL [
+    PROVE_TAC [],
+    PROVE_TAC [NOT_MEM_Delete1_IDENT],
+    PROVE_TAC []
+  ]);
+
+val Fold1_RSP = store_thm(
+  "Fold1_RSP",
+  ``!A B:'a list f (z:'b). leq A B ==> (Fold1 f z A = Fold1 f z B)``,
+  REWRITE_TAC [leq_def] THEN Induct THEN SRW_TAC [][Fold1_def] THENL [
+    PROVE_TAC [],
+    `MEM h B` by PROVE_TAC [] THEN
+    `Fold1 f z B = f h (Fold1 f z (B Delete1 h))`
+       by PROVE_TAC [MEM_lcommuting_Fold1] THEN
+    SRW_TAC [][] THEN AP_TERM_TAC THEN
+    FIRST_X_ASSUM MATCH_MP_TAC THEN SRW_TAC [][MEM_Delete1] THEN
+    PROVE_TAC [],
+    Cases_on `B` THEN SRW_TAC [][Fold1_def]
+  ]);
+
+val APPEND_RSP = store_thm(
+  "APPEND_RSP",
+  ``!A1 A2 B1 B2:'a list. leq A1 A2 /\ leq B1 B2 ==>
+                          leq (APPEND A1 B1) (APPEND A2 B2)``,
+  SRW_TAC [][leq_def]);
+
+val Inter1_def = Define
+   `($Inter1 ([]) B = [])  /\
+    ($Inter1 ((a:'a) :: A) B = if MEM a B then a :: ($Inter1 A B)
+                                          else $Inter1 A B)`;
+
+val _ = add_infix ("Inter1", 600, HOLgrammars.LEFT);
+
+val MEM_Inter1 = store_thm
+   ("MEM_Inter1",
+    ``!A B (x:'a).
+           MEM x (A Inter1 B) = MEM x A /\ MEM x B``,
+    Induct
+    THEN SRW_TAC [][Inter1_def]
+    THEN PROVE_TAC []
+   );
+
+val Inter1_RSP = store_thm
+   ("Inter1_RSP",
+    ``!A1 A2 B1 B2:'a list.
+           leq A1 A2 /\ leq B1 B2 ==>
+           leq (A1 Inter1 B1) (A2 Inter1 B2)``,
+    SRW_TAC [][leq_def, MEM_Inter1]);
+
+(* do the quotient *)
+val leq_equiv = save_thm("leq_equiv",
+    refl_sym_trans_equiv leq_refl leq_sym leq_trans);
+
+val equivs = [leq_equiv];
+
+
+val fnlist =
+    [{def_name="Empty_def",
+      fname="Empty",
+      func= ``[] :'a list``,
+      fixity=Prefix},
+
+     {def_name="Insert_def",
+      fname="Insert",
+      func= ``CONS :'a -> 'a list -> 'a list``,
+      fixity=Infixr 490},
+
+     {def_name="In_def",
+      fname="In",
+      func= ``MEM :'a -> 'a list -> bool``,
+      fixity=Infix(NONASSOC,425)},
+
+     {def_name="Card_def",
+      fname="Card",
+      func= ``Card1 :'a list -> num``,
+      fixity=Prefix},
+
+     {def_name="Delete_def",
+      fname="Delete",
+      func= ``$Delete1 :'a list -> 'a -> 'a list``,
+      fixity=Infixl 500},
+
+     {def_name="Union_def",
+      fname="Union",
+      func= ``APPEND :'a list -> 'a list -> 'a list``,
+      fixity=Infixl 500},
+
+     {def_name="Inter_def",
+      fname="Inter",
+      func= ``$Inter1 :'a list -> 'a list -> 'a list``,
+      fixity=Infixl 600},
+
+     {def_name="Fold_def",
+      fname="Fold",
+      func= ``Fold1 :('a -> 'b -> 'b) -> 'b -> 'a list -> 'b``,
+      fixity=Prefix},
+
+     {def_name="fset2set_def",
+      fname="fset2set",
+      func= ``LIST_TO_SET :'a list -> 'a -> bool``,
+      fixity=Prefix}
+    ];
+
+
+(* ==================================================== *)
+(*   LIFT TYPES, CONSTANTS, AND THEOREMS BY QUOTIENTS   *)
+(* ==================================================== *)
+
+val _ = quotient.chatting := true;   (* Causes display of quotient as built *)
+
+
+val  [finite_set_cases, Insert_LEFT_COMM, Insert_LEFT_IDEM,
+      In, NONE_In_Empty, In_Insert, finite_set_strong_cases,
+      Card, NOT_In_Card, Card_SUC, Card_Insert_GT_0,
+      In_Card_NOT_0, NOT_Empty_Insert,
+      Delete_def, In_Delete, Card_Delete,
+      Insert_Delete, In_Insert_Delete, finite_set_Delete_cases,
+      Union, In_Union, Inter, In_Inter,
+      Fold, fset2set, finite_set_EXTENSION, finite_set_INDUCT
+     ] =
+
+    define_quotient_types
+
+    {types = [{name = "finite_set", equiv = leq_equiv}],
+     defs = fnlist,
+     tyop_equivs = [],
+     tyop_quotients = [FUN_QUOTIENT],
+     tyop_simps = [FUN_REL_EQ, FUN_MAP_I],
+     respects = [NIL_RSP, CONS_RSP, MEM_RSP, Card1_RSP, Delete1_RSP,
+                 APPEND_RSP, Inter1_RSP, Fold1_RSP, list2set_RSP],
+     poly_preserves = [FORALL_PRS, EXISTS_PRS, COND_PRS],
+     poly_respects = [RES_FORALL_RSP, RES_EXISTS_RSP, COND_RSP],
+     old_thms = [list_CASES, CONS_LEFT_COMM, CONS_LEFT_IDEM,
+                 MEM, NONE_MEM_NIL, MEM_CONS, finite_set1_strong_cases,
+                 Card1_def, NOT_MEM_Card1, Card1_SUC, Card1_CONS_GT_0,
+                 MEM_Card1_NOT_0, NOT_NIL_EQUIV_CONS,
+                 Delete1_def, MEM_Delete1, Card1_Delete1,
+                 CONS_Delete1, MEM_CONS_Delete1, finite_set1_Delete1_cases,
+                 APPEND, MEM_APPEND, Inter1_def, MEM_Inter1,
+                 Fold1_def, list2set_thm, leq_def, list_INDUCT]
+   };
+
+val _ = map save_thm
+    [("finite_set_cases",finite_set_cases),
+     ("Insert_LEFT_COMM",Insert_LEFT_COMM),
+     ("Insert_LEFT_IDEM",Insert_LEFT_IDEM),
+     ("In",In),
+     ("NONE_In_Empty",NONE_In_Empty),
+     ("In_Insert",In_Insert),
+     ("finite_set_strong_cases",finite_set_strong_cases),
+     ("Card",Card),
+     ("NOT_In_Card",NOT_In_Card),
+     ("Card_SUC",Card_SUC),
+     ("Card_Insert_GT_0",Card_Insert_GT_0),
+     ("In_Card_NOT_0",In_Card_NOT_0),
+     ("NOT_Empty_Insert",NOT_Empty_Insert),
+     ("Delete_def",Delete_def),
+     ("In_Delete",In_Delete),
+     ("Card_Delete",Card_Delete),
+     ("Insert_Delete",Insert_Delete),
+     ("In_Insert_Delete",In_Insert_Delete),
+     ("finite_set_Delete_cases",finite_set_Delete_cases),
+     ("Union",Union),
+     ("In_Union",In_Union),
+     ("Inter",Inter),
+     ("In_Inter",In_Inter),
+     ("Fold",Fold),
+     ("fset2set",fset2set),
+     ("finite_set_EXTENSION",finite_set_EXTENSION),
+     ("finite_set_INDUCT",finite_set_INDUCT)
+    ];
+
+val _ = export_theory();
+
+val _ = html_theory "ext_finite_set";
